itreeS/Basics.v
@@ -1,0 +1,101 @@
+(** * General-purpose definitions *)
+
+(** Not specific to itrees. *)
+
+(* begin hide *)
+From Stdlib Require
+     Ensembles.
+
+From Stdlib Require Import
+     RelationClasses.
+
+From ExtLib Require Import
+     Structures.Functor
+     Structures.Monad
+     Data.Monads.StateMonad
+     Data.Monads.ReaderMonad
+     Data.Monads.OptionMonad
+     Data.Monads.EitherMonad.
+
+Import
+  FunctorNotation
+  MonadNotation.
+Local Open Scope monad.
+(* end hide *)
+
+(** ** Parametric functions *)
+
+(** A notation for a certain class of parametric functions.
+    Some common names of things that can be represented by such a type:
+
+    - Natural transformations (functor morphisms)
+    - Monad morphisms
+    - Event morphisms (if [E] and [F] are simply
+      indexed types with no particular structure)
+    - Event handlers (if [F] is a monad)
+ *)
+
+(** ** Common monads and transformers. *)
+
+Module Monads.
+
+Definition identity (a : Type) : Type := a.
+
+Definition stateT (S : Type) (M: Type -> Type) (A : Type) : Type :=
+  S -> M (S * A)%type.
+
+#[global] Instance Functor_stateT {M: Type -> Type} {S: Type} {Fm : Functor M} : Functor (stateT S M)
+  := {|
+    fmap _ _ f := fun run s => fmap (fun sa => (fst sa, f (snd sa))) (run s)
+    |}.
+
+#[global] Instance Monad_stateT {M: Type -> Type} {S: Type} {Fm : Monad M} : Monad (stateT S M)
+  := {|
+    ret _ a := fun s => ret (s, a)
+  ; bind _ _ t k := fun s =>
+      sa <- t s ;;
+      k (snd sa) (fst sa)
+    |}.
+
+End Monads.
+
+(** ** Loop operator *)
+
+(** [iter]: A primitive for general recursion.
+    Iterate a function updating an accumulator [I], until it produces
+    an output [R].
+ *)
+Class MonadIter (M : Type -> Type) :=
+  iter : forall {I R: Type}, (I -> M (I + R)%type) -> I -> M R.
+
+#[global] Hint Mode MonadIter ! : typeclass_instances.
+
+(** *** Transformer instances *)
+
+(** And the standard transformers can lift [iter].
+
+    Quite easily in fact, no [Monad] assumption needed.
+ *)
+
+#[global] Instance MonadIter_stateT {M: Type -> Type} {S: Type} {MM : Monad M} {AM : MonadIter M}
+  : MonadIter (Monads.stateT S M)
+  :=
+  fun _ _ step i s =>
+    iter (fun si =>
+      let s := fst si in
+      let i := snd si in
+      si' <- step i s;;
+      ret match snd si' with
+          | inl i' => inl (fst si', i')
+          | inr r => inr (fst si', r)
+          end) (s, i).
+
+Notation iEvent := (Type -> Type).
+
+Notation "E ~> F" := (forall T, E T -> F T)
+  (at level 99, right associativity, only parsing) : type_scope.
+(* The same level as [->]. *)
+(* This might actually not be such a good idea. *)
+
+(** Identity morphism. *)
+Definition idM {E : iEvent} : E ~> E := fun _ e => e.
