itreeS/CategoryOps.v
@@ -1,0 +1,212 @@
+(** * Category operations *)
+
+(** Interfaces for programming with categories. *)
+
+(** A category is represented by a type of objects [obj], and a type
+    of morphisms [C : obj -> obj -> Type].
+
+    The interface gives the signatures for the following operations
+    (which may be defined independently).
+    For any [a], [b], [c]):
+
+    - [eq2 : C a b -> C a b -> Prop], equivalence of morphisms;
+
+    - [id_ a : C a a], the identity morphism;
+    - [cat : C a b -> C b c -> C a c], composition of morphisms;
+
+    - [empty : C i a], the initial morphism (where [i] is the initial
+      object);
+
+    - [bimap : C a b -> C c d -> C (bif a b) (bif c d)], "vertical
+      composition" of morphisms, where [bif] is a bifunctor
+      (in our case it is the coproduct bifunctor);
+    - [assoc_l], [assoc_r], [unit_l], [unit_l'], [unit_r], [unit_r']:
+      natural isomorphisms of a tensor product [bif], making [C] a
+      monoidal category;
+
+    - [case_ : C a c -> C b c -> C (bif a b) c], "case analysis"
+      of a coproduct [bif];
+    - [inl_ : C a (bif a b)], left injection in a coproduct [bif];
+    - [inr_ : C b (bif a b)], right injection;
+
+    - [iter : C a (bif a b) -> C a b], loop operator.
+ *)
+
+(** We use typeclasses to give such "canonical names" to these
+    operations, allowing us to define common notations and equations
+    once and for all. This is the approach described in
+    "Type Classes for Mathematics in Type Theory",
+    by Bas Spitters and Eelis van der Weegen
+    (https://arxiv.org/abs/1102.1323).
+
+    The properties of these operations are given in
+    [Basics.CategoryTheory].
+ *)
+
+(** Notations [>>>] and [⩯] are in the module [CatNotations], under the scope
+    [cat]. The common way to use them is:
+[[
+  Import CatNotations.
+  Local Open Scope cat.
+]]
+ *)
+
+(** ** Low-level infrastructure *)
+
+(** Categories are parameterized by a type of objects [obj]. *)
+
+Module Import Carrier.
+
+(** A category will be designated by the type of its morphisms (Hom-sets),
+    which is indexed by two objects. *)
+(* Notation Hom obj := (obj -> obj -> Type) (only parsing). *)
+
+(** Examples found in this library:
+
+    - The category of functions: [obj := Type], [Fun a b := a -> b].
+    - The category of indexed functions: [obj := Type -> Type], [IFun E F := E ~> F]
+      (where [~>] is defined in [Basics.Basics]).
+    - The category of [itree] continuations (one category for every [E : Type -> Type]):
+      [obj := Type], [ktree E a b := a -> itree E a b].
+    - The category of [itree] handlers: [obj := Type -> Type],
+      [Handler E F := E ~> itree F].
+
+    The latter two are Kleisli categories of the former two respectively.
+*)
+
+(** Bifunctors from a category to itself are designated by their object maps.
+    They are associated to morphism maps via the [Bimap] class. *)
+Notation binop obj := (obj -> obj -> obj) (only parsing).
+
+End Carrier.
+
+(** Scope for category notations. *)
+Declare Scope cat_scope.
+Delimit Scope cat_scope with cat.
+
+(** ** Categories *)
+
+(* [/ᐠ｡‸｡ᐟ\] *)
+Section CatOps.
+
+  Context {obj : Type} (C : obj -> obj -> Type).
+
+(** The identity morphism for the object [a : obj] is written [id_ a]. *)
+Class Id_ : Type :=
+  id_ : forall a: obj, C a a.
+(* We add an underscore [id_] to avoid clashing with the standard
+   library [id]. *)
+
+(** Given two morphisms [f] and [g] with a common endpoint, their
+    composition (or con(cat)enation) is written [cat f g] or [f >>> g]. *)
+Class Cat : Type : Type :=
+  cat : forall a b c, C a b -> C b c -> C a c.
+
+(** If there is an initial object [i], its initial morphisms are written
+    [empty : C i a]. *)
+Class Initial (i : obj) :=
+  empty : forall a, C i a.
+
+End CatOps.
+
+Arguments id_ {obj C Id_}.
+Arguments cat {obj C Cat a b c}.
+Arguments empty {obj C i Initial a}.
+
+(** ** Bifunctors *)
+
+Section CocartesianOps.
+
+Context {obj : Type} (C : obj -> obj -> Type) (bif : binop obj).
+
+(** *** Coproducts *)
+
+(** Coproducts are a generalization of sum types and case analysis. *)
+
+(** Case analysis on a sum. *)
+Class Case :=
+  case_ : forall a b c, C a c -> C b c -> C (bif a b) c.
+
+(** Injection into the left component. *)
+Class Inl :=
+  inl_ : forall a b, C a (bif a b).
+
+(** Injection into the right component. *)
+Class Inr :=
+  inr_ : forall a b, C b (bif a b).
+
+(* Like [id_], the underscores avoid confusion with the names
+   from the stdlib ([inl] and [inr] are constructors of [sum],
+   and [case] is a tactic.) *)
+
+End CocartesianOps.
+
+Arguments case_ {obj C bif Case a b c}.
+Arguments inl_ {obj C bif Inl a b}.
+Arguments inr_ {obj C bif Inr a b}.
+
+(** ** Core notations *)
+Module Import CatNotations.
+
+Infix ">>>" := cat (at level 50, left associativity) : cat_scope.
+
+End CatNotations.
+
+Local Open Scope cat.
+
+(** ** Automatic solver of reassociating sums *)
+
+Section RESUM.
+
+Context {obj : Type} (C : obj -> obj -> Type) (bif : binop obj).
+Context `{Id_ _ C} `{Cat _ C}.
+Context `{Case _ C bif} `{Inl _ C bif} `{Inr _ C bif}.
+
+Class ReSum (a b : obj) :=
+  resum : C a b.
+
+(** The instance weights on [ReSum_inl] (8) and [ReSum_inr] (9) are so that,
+    if you have a list [E +' E +' F] (associated to the right:
+    [E +' (E +' F)]), then the first one will be picked for the inclusion
+    [E -< E +' E +' F]. *)
+
+#[global]
+Instance ReSum_id a : ReSum a a := { resum := id_ a }.
+#[global]
+Instance ReSum_sum a b c
+         `{ReSum a c} `{ReSum b c} : ReSum (bif a b) c :=
+  { resum := case_ resum resum }.
+#[global]
+Instance ReSum_inl a b c `{ReSum a b} : ReSum a (bif b c) | 8 :=
+  { resum := resum >>> inl_ }.
+#[global]
+Instance ReSum_inr a b c `{ReSum a b} : ReSum a (bif c b) | 9 :=
+  { resum := resum >>> inr_ }.
+#[global]
+Instance ReSum_empty {i : obj} `{Initial _ _ i} a : ReSum i a :=
+  { resum := empty }.
+
+(* Usage template:
+
+[[
+Opaque cat.
+Opaque id.
+Opaque case_.
+Opaque inl_.
+Opaque inr_.
+
+    (* where the category is (->)  vv *)
+Definition f {X Y Z} : complex_sum -> another_complex_sum :=
+  Eval compute in resum.
+
+Transparent cat.
+Transparent id.
+Transparent case_.
+Transparent inl_.
+Transparent inr_.
+]]
+*)
+
+End RESUM.
+
+#[global] Hint Mode ReSum ! ! ! ! : typeclass_instances.
