itreeS/Subevent.v
@@ -1,0 +1,132 @@
+(** * Extensible effects *)
+
+(** Notations to handle large sums and classes for extensible effects. *)
+
+(* begin hide *)
+From ITreeS Require Import
+     CategoryOps
+     Basics
+     Sum
+     ITreeDefinition.
+
+(* end hide *)
+
+(** Automatic application of commutativity and associativity for
+    sums types constructed with [sum1].
+
+    N.B. This is prone to infinite instance resolution loops.
+    Put the following option at the top of your [.v] files to
+    bound the instance search depth:
+
+[[
+  Typeclasses eauto := 5.
+]]
+
+    Higher numbers allow bigger instances but grow the search
+    space exponentially.
+ *)
+
+
+(** The name of the category. *)
+Definition IFun (E F : iEvent) : Type := E ~> F.
+
+(** The identity function. *)
+#[global] Instance Id_IFun : Id_ IFun := fun E _ e => e.
+
+(** Function composition. *)
+#[global] Instance Cat_IFun : Cat IFun :=
+  fun E F G f1 f2 R e => f2 _ (f1 _ e).
+
+(** [void1] is the initial object. *)
+#[global] Instance Initial_void1 : Initial IFun void1 := @elim_void1.
+
+#[global] Instance Case_sum1 : Case IFun sum1 := @case_sum1.
+#[global] Instance Inl_sum1 : Inl IFun sum1 := @inl1.
+#[global] Instance Inr_sum1 : Inr IFun sum1 := @inr1.
+
+
+
+Notation Subevent E F := (@ReSum _ IFun E F)
+  (only parsing).
+Notation "E -< F" := (Subevent E F)
+  (at level 92, left associativity) : type_scope.
+
+Definition subevent {E F : iEvent} `{E -< F} : E ~> F :=
+  resum IFun.
+
+#[global]
+Instance Subevent_refl E : @ReSum _ IFun E E.
+Proof. repeat red; eauto. Defined.
+
+(** Notations to construct and pattern-match on nested sums. *)
+Module Import SumNotations.
+
+Declare Scope sum_scope.
+Delimit Scope sum_scope with sum.
+Bind Scope sum_scope with sum1.
+
+Notation "(| x )" := (inr1 x) : sum_scope.
+Notation "( x |)" := (inl1 x) : sum_scope.
+Notation "(| x |)" := (inr1 (inl1 x)) : sum_scope.
+Notation "(|| x )" := (inr1 (inr1 x)) : sum_scope.
+Notation "(|| x |)" := (inr1 (inr1 (inl1 x))) : sum_scope.
+Notation "(||| x )" := (inr1 (inr1 (inr1 x))) : sum_scope.
+Notation "(||| x |)" := (inr1 (inr1 (inr1 (inl1 x)))) : sum_scope.
+Notation "(|||| x )" := (inr1 (inr1 (inr1 (inr1 x)))) : sum_scope.
+Notation "(|||| x |)" :=
+  (inr1 (inr1 (inr1 (inr1 (inl1 x))))) : sum_scope.
+Notation "(||||| x )" :=
+  (inr1 (inr1 (inr1 (inr1 (inr1 x))))) : sum_scope.
+Notation "(||||| x |)" :=
+  (inr1 (inr1 (inr1 (inr1 (inr1 (inl1 x)))))) : sum_scope.
+Notation "(|||||| x )" :=
+  (inr1 (inr1 (inr1 (inr1 (inr1 (inr1 x)))))) : sum_scope.
+Notation "(|||||| x |)" :=
+  (inr1 (inr1 (inr1 (inr1 (inr1 (inr1 (inl1 x))))))) : sum_scope.
+Notation "(||||||| x )" :=
+  (inr1 (inr1 (inr1 (inr1 (inr1 (inr1 (inr1 x))))))) : sum_scope.
+
+End SumNotations.
+
+Local Open Scope sum_scope.
+
+(** A polymorphic version of [Vis]. *)
+Notation vis e k := (Vis (subevent _ e) k).
+
+(* Called [send] in Haskell implementations of Freer monads. *)
+Notation trigger e := (ITree.trigger (subevent _ e)).
+
+(* Some rewriting lemmas sometimes expose [resum]. The following lemmas help reshape the goal properly *)
+Lemma resum_to_subevent : forall (E F : iEvent) H T e,
+    @resum _ IFun E F H T e = subevent _ e.
+Proof.
+  intros; reflexivity.
+Qed.
+
+Lemma subevent_subevent' : forall {E F} `{E -< F} {X} (e : E X),
+    @subevent F F _ X (@subevent E F _ X e) = subevent X e.
+Proof.
+  reflexivity.
+Qed.
+
+Lemma subevent_subevent : forall {E F G} (SEF: E -< F) (SFG: F -< G) T (e : E T),
+    @subevent F G SFG T (@subevent E F SEF T e) =
+    @subevent E G (fun x f => SFG _ (SEF _ f)) T e.
+Proof.
+  reflexivity.
+Qed.
+
+#[global] Instance subevent_void1 E: @ReSum _ IFun void1 E :=
+  fun T e => match e with end.
+
+Lemma subevent_left {E F: iEvent} {R: Type} (e: E R):
+  @subevent E (E +' F) (ReSum_inl _ _ _ _ _) R e = inl1 e.
+Proof.
+  reflexivity.
+Qed.
+
+Lemma subevent_right {E F: iEvent} {R: Type} (e: F R):
+  @subevent F (E +' F) (ReSum_inr _ _ _ _ _) R e = inr1 e.
+Proof.
+  reflexivity.
+Qed.
