itreeS/Sum.v
@@ -1,0 +1,43 @@
+(** * Sums of indexed types *)
+
+(** In the context of interaction trees, events can be combined
+    using this sum type. *)
+
+(* begin hide *)
+
+From ITreeS Require Import Basics.
+
+Set Implicit Arguments.
+Set Contextual Implicit.
+
+(* end hide *)
+
+(** Sum of type constructors [Type -> Type].
+
+    [sum1 : (Type -> Type) -> (Type -> Type) -> (Type -> Type)]. *)
+Variant sum1 (E1 E2 : iEvent) (X : Type) : Type :=
+| inl1 (_ : E1 X)
+| inr1 (_ : E2 X).
+Arguments inr1 {E1 E2} [X].
+Arguments inl1 {E1 E2} [X].
+
+(** An infix notation for convenience. *)
+Notation "E1 +' E2" := (sum1 E1 E2)
+  (at level 59, right associativity) : type_scope.
+
+(** The coproduct is case analysis on sums. *)
+Definition case_sum1 {A B C : iEvent} (f : A ~> C) (g : B ~> C)
+  : A +' B ~> C
+  := fun _ ab =>
+       match ab with
+       | inl1 a => f _ a
+       | inr1 b => g _ b
+       end.
+
+(** The empty indexed type. *)
+Variant void1 : Type -> Type := .
+
+(* Eliminate [void1]. *)
+Definition elim_void1 {E: iEvent}
+  : forall T : Type, void1 T -> E T :=
+  fun T (v : void1 T) => match v with end.
